corrected defn of mgu

mgu.fst
@@ -9,19 +9,36 @@ let rec apply_tuple_list st l = match l with
   | [] -> []
   | (hd1,hd2)::tl -> (apply st hd1 , apply st hd2)::(apply_tuple_list st tl)
 
+val apply_list_length_lemma : st:subst -> l:list (term*term) -> Lemma
+  (requires true)
+  (ensures ( List.Tot.length l = List.Tot.length (apply_tuple_list st l)) )
+
+let rec apply_list_length_lemma st l = match l with
+  | [] -> ()
+  | hd::tl -> apply_list_length_lemma st tl
+
+val collate : l1:list term -> l2:list term {List.Tot.length l1 = List.Tot.length l2}-> Tot (list (term*term))
+
+let rec collate l1 l2 = match l1,l2 with
+  | [],[] -> []
+  | hd1::tl1,hd2::tl2 -> (hd1,hd2)::(collate tl1 tl2)
+
 val sub_mgu : l:list (term*term) -> st:subst -> Tot (option subst)
 let rec sub_mgu l st = match l with
   | [] -> Some st
   | (Var v, x)::tl -> begin
                         let temp1 = (compose st [(v,x)]) in
                         let temp2 = (apply_tuple_list [(v,x)] tl) in
+                        apply_list_length_lemma st tl;
                         if None? (sub_mgu temp2 temp1) then None
                         else (sub_mgu temp2 temp1)
                       end
   | (x,Var v)::tl -> begin
                         let temp1 = (compose st [(v,x)]) in
                         let temp2 = (apply_tuple_list [(v,x)] tl) in
+                        apply_list_length_lemma st tl;
                         if None? (sub_mgu temp2 temp1) then None
                         else (sub_mgu temp2 temp1)
                      end
+  | (Func s args1, Func s args2)::tl -> sub_mgu (List.Tot.append (collate args1 args2) tl) st
   | _ -> None
